Minor layout tweak on AsCif

nola/iris/cif.v
@@ -464,8 +464,7 @@ Section cif_ecustom.
 End cif_ecustom.
 
 (** ** [AsCif]: Reify [iProp] into [cif] *)
-Class AsCif `{!Csem CON JUDG Σ} (Φ : (JUDG -n> iProp Σ) → iProp Σ) :=
-  AS_CIF {
+Class AsCif `{!Csem CON JUDG Σ} (Φ : (JUDG -n> iProp Σ) → iProp Σ) := AS_CIF {
   as_cif : cif CON Σ;
   sem_as_cif {δ} : cif_sem δ as_cif ⊣⊢ Φ δ;
 }.
@@ -485,24 +484,19 @@ Section as_cif.
   #[export] Program Instance ex_as_cif `{!∀ a : A, AsCif CON (Φ a)} :
     AsCif CON (λ δ, ∃ a : A, Φ a δ)%I | 5 := AS_CIF (∃ a, as_cif (Φ a)) _.
   Next Obligation. move=>/= *. f_equiv=> ?. exact sem_as_cif. Qed.
-  #[export] Program Instance and_as_cif
-    `{!AsCif CON Φ, !AsCif CON Ψ} :
+  #[export] Program Instance and_as_cif `{!AsCif CON Φ, !AsCif CON Ψ} :
     AsCif CON (λ δ, Φ δ ∧ Ψ δ)%I | 5 := AS_CIF (as_cif Φ ∧ as_cif Ψ) _.
   Next Obligation. move=>/= *. f_equiv; exact sem_as_cif. Qed.
-  #[export] Program Instance or_as_cif
-    `{!AsCif CON Φ, !AsCif CON Ψ} :
+  #[export] Program Instance or_as_cif `{!AsCif CON Φ, !AsCif CON Ψ} :
     AsCif CON (λ δ, Φ δ ∨ Ψ δ)%I | 5 := AS_CIF (as_cif Φ ∨ as_cif Ψ) _.
   Next Obligation. move=>/= *. f_equiv; exact sem_as_cif. Qed.
-  #[export] Program Instance imp_as_cif
-    `{!AsCif CON Φ, !AsCif CON Ψ} :
+  #[export] Program Instance imp_as_cif `{!AsCif CON Φ, !AsCif CON Ψ} :
     AsCif CON (λ δ, Φ δ → Ψ δ)%I | 5 := AS_CIF (as_cif Φ → as_cif Ψ) _.
   Next Obligation. move=>/= *. f_equiv; exact sem_as_cif. Qed.
-  #[export] Program Instance sep_as_cif
-    `{!AsCif CON Φ, !AsCif CON Ψ} :
+  #[export] Program Instance sep_as_cif `{!AsCif CON Φ, !AsCif CON Ψ} :
     AsCif CON (λ δ, Φ δ ∗ Ψ δ)%I | 5 := AS_CIF (as_cif Φ ∗ as_cif Ψ) _.
   Next Obligation. move=>/= *. f_equiv; exact sem_as_cif. Qed.
-  #[export] Program Instance wand_as_cif
-    `{!AsCif CON Φ, !AsCif CON Ψ} :
+  #[export] Program Instance wand_as_cif `{!AsCif CON Φ, !AsCif CON Ψ} :
     AsCif CON (λ δ, Φ δ -∗ Ψ δ)%I | 5 := AS_CIF (as_cif Φ -∗ as_cif Ψ) _.
   Next Obligation. move=>/= *. f_equiv; exact sem_as_cif. Qed.
   #[export] Program Instance plain_as_cif `{!AsCif CON Φ} :
